Valaig/Aiger.lean
@@ -1,4 +1,3 @@
 import Valaig.Aiger.Basic
-import Valaig.Aiger.Lemmas
 import Valaig.Aiger.Parser
 import Valaig.Aiger.Writer
